src/program_proof/pb/append_proof.v
@@ -1,11 +1,210 @@
 From Perennial.program_proof Require Import grove_prelude.
 From Goose.github_com.mit_pdos.gokv Require Import pb.
 
-From Perennial.program_proof.pb Require Export common_proof append_marshal_proof replica_defns.
+From Perennial.program_proof.pb Require Export common_proof append_marshal_proof replica_defns replica_ghost_proof.
 
 Section append_proof.
 
 Context `{!heapGS Σ}.
+
+Lemma wp_ReplicaServer__AppendRPC (s:loc) rid γ (args_ptr:loc) args :
+  {{{
+       "#HisRepl" ∷ is_ReplicaServer s rid γ ∗
+       "Hargs" ∷ own_AppendArgs args_ptr args ∗
+       "#Hproposal_lb_in" ∷ proposal_lb γ args.(AA_cn) args.(AA_log) ∗
+       "#HoldConfMax_in" ∷ oldConfMax γ args.(AA_cn) args.(AA_log) ∗
+       "#Hcommit_lb_in" ∷ commit_lb_by γ args.(AA_cn) (take (int.nat args.(AA_commitIdx)) args.(AA_log)) ∗
+       "%HcommitLength" ∷ ⌜int.Z args.(AA_commitIdx) < length args.(AA_log)⌝
+  }}}
+    ReplicaServer__AppendRPC #s #args_ptr
+  {{{
+       (r:bool), RET #r; ⌜r = true⌝ ∗ accepted_lb γ args.(AA_cn) rid args.(AA_log) ∨ ⌜r = false⌝
+  }}}
+.
+Proof.
+  iIntros (Φ) "Hpre HΦ".
+  iNamed "Hpre".
+  iNamed "HisRepl".
+  wp_lam.
+  wp_pures.
+  wp_loadField.
+  wp_apply (acquire_spec with "HmuInv").
+  iIntros "[Hlocked Hown]".
+  iNamed "Hown".
+
+  wp_pures.
+  iNamed "Hargs".
+  (* First, deal with the replica step for appendRPC *)
+  iNamed "Hrep".
+  wp_loadField.
+  wp_loadField.
+
+  wp_if_destruct.
+  { (* case: args.cn < s.cn *)
+    wp_loadField.
+    wp_apply (release_spec with "[-HΦ]").
+    {
+      iFrame "HmuInv Hlocked". iNext.
+      do 6 iExists _.
+      iFrame "∗#".
+      iExists _; iFrame.
+    }
+    wp_pures.
+    iApply "HΦ".
+    iRight.
+    done.
+  }
+
+  (* case: args.cn ≥ s.cn *)
+  wp_loadField.
+  wp_loadField.
+  wp_apply (wp_or with "[HopLog HAlog]").
+  { iNamedAccu. }
+  { by wp_pures. }
+  {
+    iIntros "% HH"; iNamed "HH".
+    wp_loadField.
+    wp_apply (wp_slice_len).
+    wp_loadField.
+    wp_apply (wp_slice_len).
+    wp_pures.
+    by iFrame.
+  }
+  iNamed 1.
+
+  iDestruct (is_slice_sz with "HopLog_slice") as %HopLogLen.
+  iDestruct (is_slice_sz with "HAlog_slice") as %HALogLen.
+  wp_apply (wp_If_join_evar with "[HopLog HopLog_slice Hcn HAlog HAlog_slice HAcn HrepG]").
+  {
+    iIntros.
+    wp_if_destruct; last first.
+    { (* won't grow log *)
+      iMod (append_dup_ghost with "[$HrepG $Hproposal_lb_in]") as "[HrepG #Hacc]".
+      { word. }
+
+      iModIntro; iSplitL ""; first done.
+      iAssert (∃ r',
+                  "Hrep" ∷ own_Replica_phys s r' ∗
+                  "HrepG" ∷ own_Replica_ghost rid γ r'
+              )%I with "[HopLog HopLog_slice Hcn HrepG]" as "HH".
+      {
+        iExists _; iFrame. iExists _; iFrame.
+      }
+      iClear "HAlog HAcn HAlog_slice".
+      iNamedAccu.
+    }
+    { (* will grow the log *)
+      wp_loadField.
+      wp_apply (wp_storeField with "HopLog").
+      { apply slice_val_ty. }
+      iIntros "HopLog".
+      wp_pures.
+      wp_loadField.
+      wp_apply wp_fupd.
+      wp_storeField.
+      iSplitL ""; first done.
+      iExists (mkReplica _ _).
+      iSplitL "Hcn HopLog HAlog_slice".
+      { (* re-establish own_Replica_phys *)
+        iExists _. simpl. iFrame. done.
+      }
+      iMod (append_new_ghost with "[$HrepG $Hproposal_lb_in]") as "[$ #Hacc]".
+      { word. }
+      done.
+    }
+  }
+  (* Done with replica step *)
+
+  (* Do committer step *)
+  iIntros "HH".
+  wp_loadField.
+  wp_loadField.
+
+  wp_pures.
+  iClear "Hproposal_lb HoldConfMax".
+  iRename "Hcommit_lb" into "Hcommit_lb_old".
+  iNamed "HH".
+  iNamed "HH".
+  wp_apply (wp_If_join_evar with "[HcommitIdx HAcommitIdx]").
+  {
+    iIntros.
+    wp_if_destruct.
+    { (* args.commitIdx > commitIdx *)
+      wp_loadField.
+      wp_storeField.
+      iSplitL ""; first done.
+      iAssert (∃ (commitIdx':u64), "Hcommit" ∷ s ↦[ReplicaServer :: "commitIdx"] #commitIdx' ∗
+                                   "#Hcommit_lb" ∷ commit_lb_by γ args.(AA_cn) (take (int.nat commitIdx') opLog') ∗
+                                   "%HcommitLeLogLen" ∷ ⌜int.Z commitIdx' ≤ length opLog'⌝
+              )%I with "[HcommitIdx]" as "HH".
+      {
+        iExists _.
+        iFrame.
+        (* prove that args.(AA_log) ≤ opLog' or that
+           opLog' ≤ args.(AA_log);
+         *)
+        (* Use the fact that args.(AA_log) and opLog' are comparable. *)
+        assert ( take (int.nat args.(AA_commitIdx)) opLog' ⪯
+                (take (int.nat args.(AA_commitIdx)) args.(AA_log)))%I.
+        {
+          set (l1:=args.(AA_log)) in *.
+          set (l2:=opLog') in *.
+          set (e:=int.nat args.(AA_commitIdx)) in *.
+          assert (e < length l1) by word.
+          clear -H0 HnewLog.
+          admit. (* TODO: pure list fact *)
+        }
+        iSplitR "".
+        {
+          iApply (commit_lb_by_monotonic with "Hcommit_lb_in").
+          { word. }
+          done.
+        }
+        {
+          iPureIntro.
+          assert (length args.(AA_log) ≤ length opLog').
+          { admit. (* TODO: pure fact *) }
+          word.
+        }
+      }
+      iNamedAccu.
+    }
+    { (* args.commitIdx is not larger than commitIdx. boils down to the newly
+         proposed value not contradicting the previously committed stuff, the
+         proof is done earlier for conveneince. *)
+        iModIntro. iSplitL ""; first done.
+        iFrame.
+        iExists commitIdx.
+        iFrame.
+        iFrame "#".
+        {
+          iPureIntro.
+          assert (length args.(AA_log) ≤ length opLog').
+          { admit. (* TODO: pure fact *) }
+          word.
+        }
+    }
+  }
+  iIntros "HH".
+  iNamed "HH".
+  iNamed "HH".
+  wp_pures.
+  wp_storeField.
+  wp_loadField.
+  wp_apply (release_spec with "[-HΦ]").
+  {
+    iFrame "HmuInv Hlocked".
+    iNext.
+    do 9 iExists _.
+    iFrame "∗#".
+    done.
+  }
+  wp_pures.
+  iApply "HΦ".
+  iLeft.
+  iFrame "#".
+  by iModIntro.
+Admitted.
 
 Lemma wp_ReplicaServer__postAppendRPC (s:loc) (i:u64) conf rid γ (args_ptr:loc) args :
   {{{
@@ -34,6 +233,9 @@ Proof.
   wp_pures.
   iNamed "Hown".
   iNamed "Hargs".
+
+  (* First, deal with the replica step. *)
+  iNamed "Hrep".
   wp_loadField.
   wp_loadField.
   wp_if_destruct; last first.
@@ -44,9 +246,8 @@ Proof.
     {
       iFrame "HmuInv Hlocked".
       iNext.
-      do 9 iExists _. iFrame "∗ #".
-      iFrame "Hown".
-      done.
+      do 6 iExists _. iFrame "∗ #".
+      iExists _; iFrame.
     }
     wp_pures.
     by iApply "HΦ".
@@ -161,302 +362,6 @@ Proof.
     wp_pures.
     by iApply "HΦ".
   }
-Admitted.
-
-Lemma wp_ReplicaServer__AppendRPC (s:loc) rid γ (args_ptr:loc) args :
-  {{{
-       "#HisRepl" ∷ is_ReplicaServer s rid γ ∗
-       "Hargs" ∷ own_AppendArgs args_ptr args ∗
-       "#Hproposal_lb_in" ∷ proposal_lb γ args.(AA_cn) args.(AA_log) ∗
-       "#HoldConfMax_in" ∷ oldConfMax γ args.(AA_cn) args.(AA_log) ∗
-       "#Hcommit_lb_in" ∷ commit_lb_by γ args.(AA_cn) (take (int.nat args.(AA_commitIdx)) args.(AA_log)) ∗
-       "%HcommitLength" ∷ ⌜int.Z args.(AA_commitIdx) < length args.(AA_log)⌝
-  }}}
-    ReplicaServer__AppendRPC #s #args_ptr
-  {{{
-       (r:bool), RET #r; ⌜r = true⌝ ∗ accepted_lb γ args.(AA_cn) rid args.(AA_log) ∨ ⌜r = false⌝
-  }}}
-.
-Proof.
-  iIntros (Φ) "Hpre HΦ".
-  iNamed "Hpre".
-  iNamed "HisRepl".
-  wp_lam.
-  wp_pures.
-  wp_loadField.
-  wp_apply (acquire_spec with "HmuInv").
-  iIntros "[Hlocked Hown]".
-  iNamed "Hown".
-
-  wp_pures.
-  iNamed "Hargs".
-  wp_loadField.
-  wp_loadField.
-
-  wp_if_destruct.
-  { (* args.cn < s.cn *)
-    wp_loadField.
-    wp_apply (release_spec with "[-HΦ]").
-    {
-    iFrame "HmuInv Hlocked". iNext.
-    iExists _, _, _, _, _, _, _, _.
-    iExists _. (* can only iExists 8 things at a time *)
-    iFrame "∗#".
-    iFrame "Hown".
-    done.
-    }
-    wp_pures.
-    iApply "HΦ".
-    iRight.
-    done.
-  }
-  (* args.cn ≥ s.cn *)
-
-  wp_loadField.
-  wp_loadField.
-  wp_apply (wp_or with "[HopLog HAlog]").
-  { iNamedAccu. }
-  { by wp_pures. }
-  {
-    iIntros "% HH"; iNamed "HH".
-    wp_loadField.
-    wp_apply (wp_slice_len).
-    wp_loadField.
-    wp_apply (wp_slice_len).
-    wp_pures.
-    by iFrame.
-  }
-  iNamed 1.
-
-  iDestruct (is_slice_sz with "HopLog_slice") as %HopLogLen.
-  iDestruct (is_slice_sz with "HAlog_slice") as %HALogLen.
-  wp_apply (wp_If_join_evar with "[Haccepted HacceptedUnused HopLog HopLog_slice Hcn HAlog HAlog_slice HAcn]").
-  {
-    iIntros.
-    wp_if_destruct; last first.
-    { (* won't grow log *)
-    iModIntro; iSplitL ""; first done.
-    iAssert (∃ opLog_sl' opLog',
-              "HopLog" ∷ s ↦[ReplicaServer :: "opLog"] (slice_val opLog_sl') ∗
-                       "HopLog_slice" ∷ is_slice opLog_sl' byteT 1 opLog' ∗
-                       "Haccepted" ∷ accepted_ptsto γ args.(AA_cn) rid opLog' ∗
-                       "HacceptedUnused" ∷ ([∗ set] cn_some ∈ fin_to_set u64, ⌜int.Z cn_some ≤ int.Z args.(AA_cn)⌝
-                                                                              ∨ accepted_ptsto γ cn_some rid []) ∗
-                       "#Hproposal_lb" ∷ proposal_lb γ args.(AA_cn) opLog' ∗
-                       "#HoldConfMax" ∷ oldConfMax γ args.(AA_cn) opLog' ∗
-                       "Hcn" ∷ s ↦[ReplicaServer :: "cn"] #args.(AA_cn) ∗
-                       "#Hcommit_lb_oldIdx" ∷ commit_lb_by γ args.(AA_cn) (take (int.nat commitIdx) opLog') ∗
-                       "%HnewLog" ∷ ⌜args.(AA_log) ⪯ opLog'⌝ ∗
-                       "#Hacc_lb" ∷ accepted_lb γ args.(AA_cn) rid args.(AA_log) ∗
-                       "%HcommitIdxLeNewLogLen" ∷ ⌜int.Z commitIdx ≤ length opLog'⌝
-            )%I with "[HopLog HopLog_slice Haccepted HacceptedUnused Hproposal_lb HoldConfMax Hcn]" as "HH".
-    {
-      replace (cn) with (args.(AA_cn)); last by word.
-      iDestruct (accepted_witness with "Haccepted") as "#Hacc_lb".
-      iExists _, _; iFrame "∗#".
-      assert (int.nat opLog_sl.(Slice.sz) >= int.nat log_sl.(Slice.sz))%Z as HopLogBigger.
-      { word. }
-
-      iDestruct (proposal_lb_comparable with "Hproposal_lb_in Hproposal_lb") as %Hcomparable.
-      destruct Hcomparable as [|].
-      { (* case 1: args.log ⪯ opLog *)
-        iSplitL ""; first done.
-        iSplitR ""; last done.
-        by iApply accepted_lb_monotonic.
-      }
-      { (* case 2: opLog ⪯ args.log; this will imply that the two are actually equal *)
-        rewrite -HopLogLen in HopLogBigger.
-        rewrite -HALogLen in HopLogBigger.
-        assert (opLog = args.(AA_log)) as ->.
-        { (* FIXME: pure list prefix fact *)
-          admit.
-        }
-        iFrame "#".
-        done.
-      }
-    }
-    iClear "HAlog HAcn HAlog_slice".
-    iNamedAccu.
-    }
-    { (* will grow the log *)
-      wp_loadField.
-      wp_apply (wp_storeField with "HopLog").
-      { apply slice_val_ty. }
-      iIntros "HopLog".
-      wp_pures.
-      wp_loadField.
-      wp_apply wp_fupd.
-      wp_storeField.
-      iSplitL ""; first done.
-      iExists _, _.
-      iFrame "HopLog ∗#".
-      (* TODO: Ghost stuff. *)
-      (* destruct into cases; in case we increase cn, use oldConfMax to maintain commit_lb *)
-      assert (int.Z cn > int.Z args.(AA_cn) ∨ int.Z cn = int.Z args.(AA_cn) ∨ int.Z cn < int.Z args.(AA_cn)) as Htrichotomy.
-      { word. }
-      destruct Htrichotomy as [Hbad|[Heq|HlargerLog]].
-      { exfalso. word. }
-      { (* in this case, must have len(args.log) ≥ len(s.cn) *)
-        assert (int.nat opLog_sl.(Slice.sz) < int.nat log_sl.(Slice.sz)) as HlargerLog2.
-        { word. }
-        rewrite -HopLogLen -HALogLen in HlargerLog2.
-        assert (cn = args.(AA_cn)) as -> by word.
-        iFrame "∗#".
-        iDestruct (proposal_lb_comparable with "Hproposal_lb_in Hproposal_lb") as %Hcomparable.
-        destruct Heqb0 as [Hbad|HargLogLenLarger].
-        { exfalso. word. }
-        assert (opLog ⪯ args.(AA_log)) as HargLogLarger.
-        { (* TODO: comparable + longer length -> larger log *)
-          admit. }
-        iMod (accepted_update with "Haccepted") as "Haccepted".
-        { done. }
-        iDestruct (accepted_witness with "Haccepted") as "#Hacc_lb".
-        iFrame "Hacc_lb".
-        iSplitL "Haccepted"; first done.
-        assert (take (int.nat commitIdx) args.(AA_log) ⪯ take (int.nat commitIdx) opLog).
-        { (* TODO: Use the fact that commitIdx ≤ len(opLog) to make this work *)
-          admit.
-        }
-        iSplitR "".
-        {
-          iApply (commit_lb_by_monotonic with "Hcommit_lb").
-          { done. }
-          { done. }
-        }
-        iSplitR ""; first done.
-        iPureIntro.
-        word.
-      }
-      { (* args.cn > s.cn: in this case, we want to increase our cn to args.cn *)
-        iClear "Haccepted". (* throw away the old accepted↦ *)
-        iDestruct (big_sepS_elem_of_acc_impl args.(AA_cn) with "HacceptedUnused") as "[Haccepted Hunused]".
-        { set_solver. }
-        iDestruct "Haccepted" as "[%Hbad|Haccepted]".
-        { exfalso; word. }
-        iMod (accepted_update _ _ _ _ args.(AA_log) with "Haccepted") as "Haccepted".
-        { admit. }
-        iDestruct (accepted_witness with "Haccepted") as "#Hacc_lb".
-        iSplitL "Haccepted"; first done.
-        iSplitL "Hunused".
-        {
-          iApply "Hunused".
-          {
-            iModIntro.
-            iIntros (???) "[%Hcase|Hcase]".
-            { iLeft. iPureIntro. word. }
-            { iFrame. }
-          }
-          {
-            iLeft. iPureIntro. word.
-          }
-        }
-        iFrame "Hacc_lb".
-
-        iDestruct (oldConfMax_commit_lb_by with "HoldConfMax_in Hcommit_lb") as %HlogLe.
-        { done. }
-        iSplitR ""; last first.
-        {
-          iSplitL ""; first done.
-          iPureIntro.
-          admit. (* TODO: Pure fact about lists *)
-        }
-
-        iApply (commit_lb_by_monotonic with "Hcommit_lb").
-        { word. }
-        clear -HlogLe.
-        (* TODO: pure fact about lists and prefixes *)
-        admit.
-      }
-    }
-  }
-  iIntros "HH".
-  wp_loadField.
-  wp_loadField.
-
-  wp_pures.
-  iClear "Hproposal_lb HoldConfMax".
-  iRename "Hcommit_lb" into "Hcommit_lb_old".
-  iNamed "HH".
-  iNamed "HH".
-  wp_apply (wp_If_join_evar with "[HcommitIdx HAcommitIdx]").
-  {
-    iIntros.
-    wp_if_destruct.
-    { (* args.commitIdx > commitIdx *)
-      wp_loadField.
-      wp_storeField.
-      iSplitL ""; first done.
-      iAssert (∃ (commitIdx':u64), "Hcommit" ∷ s ↦[ReplicaServer :: "commitIdx"] #commitIdx' ∗
-                                   "#Hcommit_lb" ∷ commit_lb_by γ args.(AA_cn) (take (int.nat commitIdx') opLog') ∗
-                                   "%HcommitLeLogLen" ∷ ⌜int.Z commitIdx' ≤ length opLog'⌝
-              )%I with "[HcommitIdx]" as "HH".
-      {
-        iExists _.
-        iFrame.
-        (* prove that args.(AA_log) ≤ opLog' or that
-           opLog' ≤ args.(AA_log);
-         *)
-        (* Use the fact that args.(AA_log) and opLog' are comparable. *)
-        assert ( take (int.nat args.(AA_commitIdx)) opLog' ⪯
-                (take (int.nat args.(AA_commitIdx)) args.(AA_log)))%I.
-        {
-          set (l1:=args.(AA_log)) in *.
-          set (l2:=opLog') in *.
-          set (e:=int.nat args.(AA_commitIdx)) in *.
-          assert (e < length l1) by word.
-          clear -H0 HnewLog.
-          admit. (* TODO: pure list fact *)
-        }
-        iSplitR "".
-        {
-          iApply (commit_lb_by_monotonic with "Hcommit_lb_in").
-          { word. }
-          done.
-        }
-        {
-          iPureIntro.
-          assert (length args.(AA_log) ≤ length opLog').
-          { admit. (* TODO: pure fact *) }
-          word.
-        }
-      }
-      iNamedAccu.
-    }
-    { (* args.commitIdx is not larger than commitIdx. boils down to the newly
-         proposed value not contradicting the previously committed stuff, the
-         proof is done earlier for conveneince. *)
-        iModIntro. iSplitL ""; first done.
-        iFrame.
-        iExists commitIdx.
-        iFrame.
-        iFrame "#".
-        {
-          iPureIntro.
-          assert (length args.(AA_log) ≤ length opLog').
-          { admit. (* TODO: pure fact *) }
-          word.
-        }
-    }
-  }
-  iIntros "HH".
-  iNamed "HH".
-  iNamed "HH".
-  wp_pures.
-  wp_storeField.
-  wp_loadField.
-  wp_apply (release_spec with "[-HΦ]").
-  {
-    iFrame "HmuInv Hlocked".
-    iNext.
-    do 9 iExists _.
-    iFrame "∗#".
-    done.
-  }
-  wp_pures.
-  iApply "HΦ".
-  iLeft.
-  iFrame "#".
-  by iModIntro.
 Admitted.
 
 End append_proof.
