src/program_proof/pb/replica_ghost_proof.v
@@ -1,6 +1,6 @@
 From Perennial.program_proof Require Import grove_prelude.
 From Goose.github_com.mit_pdos.gokv Require Import pb.
-From Perennial.program_proof.pb Require Export ghost_proof.
+From Perennial.program_proof.pb Require Export replica_ghost_defns.
 
 Section replica_ghost_proof.
 
@@ -8,26 +8,24 @@ Context `{!heapGS Σ}.
 Context `{!rpcregG Σ}.
 Implicit Type γ:pb_names.
 
-Lemma append_new_ghost γ r (newCn:u64) newLog :
-  "Hown" ∷ own_Replica_ghost γ r ∗
-  "#HnewProp" ∷ proposal_lb γ newCn newLog ∗
-  "%Hnew" ∷ ⌜int.Z r.(cn) < int.Z newCn ∨ r.(opLog )⪯ newLog⌝
+Lemma append_new_ghost {rid} γ r (newCn:u64) newLog :
+  int.Z r.(cn) < int.Z newCn ∨ length r.(opLog ) ≤ length newLog →
+  "Hown" ∷ own_Replica_ghost rid γ r ∗
+  "#HnewProp" ∷ proposal_lb γ newCn newLog
   ={⊤}=∗
-  accepted_lb γ newCn r.(rid) newLog.
+  own_Replica_ghost rid γ (mkReplica newLog newCn) ∗
+  accepted_lb γ newCn rid newLog.
 Proof.
-  iNamed 1.
-  iNamed "Hown".
 Admitted.
 
-Lemma append_dup_ghost γ r (newCn:u64) newLog :
-  "Hown" ∷ own_Replica_ghost γ r ∗
-  "#HnewProp" ∷ proposal_lb γ newCn newLog ∗
-  "%Hdup" ∷ ⌜int.Z r.(cn) = int.Z newCn ∧ newLog ⪯ r.(opLog )⌝
+Lemma append_dup_ghost {rid} γ r (newCn:u64) newLog :
+  int.Z r.(cn) = int.Z newCn ∧ length newLog ≤ length r.(opLog) →
+  "Hown" ∷ own_Replica_ghost rid γ r ∗
+  "#HnewProp" ∷ proposal_lb γ newCn newLog
   ={⊤}=∗
-  accepted_lb γ newCn r.(rid) newLog.
+  own_Replica_ghost rid γ r ∗
+  accepted_lb γ newCn rid newLog.
 Proof.
-  iNamed 1.
-  iNamed "Hown".
 Admitted.
 
 End replica_ghost_proof.
